@prefix : <http://example.org/ontology#> .
@prefix owl: <http://www.w3.org/2002/07/owl#> .
@prefix rdf: <http://www.w3.org/1999/02/22-rdf-syntax-ns#> .
@prefix xml: <http://www.w3.org/XML/1998/namespace> .
@prefix xsd: <http://www.w3.org/2001/XMLSchema#> .
@prefix rdfs: <http://www.w3.org/2000/01/rdf-schema#> .
@prefix time: <http://www.w3.org/2006/time#> .

<http://example.org/ontology> rdf:type owl:Ontology .

### Classes

:FilmEvent rdf:type owl:Class ;
           rdfs:label "Film Event" ;
           rdfs:comment "A class representing events where films are shown." .

:ActionFilm rdf:type owl:Class ;
            rdfs:subClassOf :FilmEvent ;
            rdfs:label "Action Film" ;
            rdfs:comment "A subclass of Film Event that is specific to action genre films." .

:Cinema rdf:type owl:Class ;
        rdfs:label "Cinema" ;
        rdfs:comment "A class representing a cinema where film events take place." .

### Object Properties

:hasStartTime rdf:type owl:ObjectProperty ;
              rdfs:domain :FilmEvent ;
              rdfs:range xsd:dateTime ;
              rdfs:label "has start time" ;
              rdfs:comment "The property that indicates the start time of a film event." .

:hasEndTime rdf:type owl:ObjectProperty ;
            rdfs:domain :FilmEvent ;
            rdfs:range xsd:dateTime ;
            rdfs:label "has end time" ;
            rdfs:comment "The property that indicates the end time of a film event." .

:takesPlaceAt rdf:type owl:ObjectProperty ;
              rdfs:domain :FilmEvent ;
              rdfs:range :Cinema ;
              rdfs:label "takes place at" ;
              rdfs:comment "The property that associates a film event with a cinema where it takes place." .

### Individuals

:CinemaOne rdf:type :Cinema ;
           rdfs:label "CinemaOne" ;
           rdfs:comment "An individual representing the CinemaOne venue." .

:XMenPreview rdf:type :ActionFilm ;
             rdfs:label "X-men Sneak Preview" ;
             :hasStartTime "2023-04-01T20:00:00"^^xsd:dateTime ;
             :takesPlaceAt :CinemaOne ;
             rdfs:comment "An individual representing the sneak preview event of the action film 'X-men'." .

### Assumptions for end time (not provided in the scenario)

:XMenPreview :hasEndTime "2023-04-01T22:00:00"^^xsd:dateTime .
