@prefix : <http://example.org/onto#> .
@prefix owl: <http://www.w3.org/2002/07/owl#> .
@prefix rdf: <http://www.w3.org/1999/02/22-rdf-syntax-ns#> .
@prefix xml: <http://www.w3.org/XML/1998/namespace> .
@prefix xsd: <http://www.w3.org/2001/XMLSchema#> .
@prefix rdfs: <http://www.w3.org/2000/01/rdf-schema#> .
@prefix agentrole: <http://www.ontologydesignpatterns.org/cp/owl/agentrole.owl#> .
@prefix objectrole: <http://www.ontologydesignpatterns.org/cp/owl/objectrole.owl#> .

<http://example.org/onto#> rdf:type owl:Ontology ;
                            rdfs:comment "An ontology for representing the context-dependent content presentation in a smart bathroom environment." .

### Classes

:User rdf:type owl:Class ;
       rdfs:subClassOf agentrole:Agent ;
       rdfs:label "User" ;
       rdfs:comment "An individual who is using the smart bathroom." .

:SmartMirror rdf:type owl:Class ;
              rdfs:label "Smart Mirror" ;
              rdfs:comment "A mirror in the smart bathroom capable of displaying graphical content." .

:SmartSpeaker rdf:type owl:Class ;
               rdfs:label "Smart Speaker" ;
               rdfs:comment "A speaker in the smart bathroom capable of reading out content." .

:Content rdf:type owl:Class ;
          rdfs:label "Content" ;
          rdfs:comment "The information content that can be presented to the user." .

:WeatherContent rdf:type owl:Class ;
                 rdfs:subClassOf :Content ;
                 rdfs:label "Weather Content" ;
                 rdfs:comment "Content that includes weather information." .

:UserLocation rdf:type owl:Class ;
               rdfs:label "User Location" ;
               rdfs:comment "The location of the user within the smart bathroom." .

:UserActivity rdf:type owl:Class ;
               rdfs:label "User Activity" ;
               rdfs:comment "The activity that the user is currently engaged in within the smart bathroom." .

### Object Properties

:hasLocation rdf:type owl:ObjectProperty ;
              rdfs:domain :User ;
              rdfs:range :UserLocation ;
              rdfs:label "has location" ;
              rdfs:comment "The current location of the user within the smart bathroom." .

:hasActivity rdf:type owl:ObjectProperty ;
              rdfs:domain :User ;
              rdfs:range :UserActivity ;
              rdfs:label "has activity" ;
              rdfs:comment "The current activity that the user is engaged in within the smart bathroom." .

:displaysContent rdf:type owl:ObjectProperty ;
                  rdfs:domain :SmartMirror ;
                  rdfs:range :Content ;
                  rdfs:label "displays content" ;
                  rdfs:comment "The smart mirror displays content." .

:readsOutContent rdf:type owl:ObjectProperty ;
                  rdfs:domain :SmartSpeaker ;
                  rdfs:range :Content ;
                  rdfs:label "reads out content" ;
                  rdfs:comment "The smart speaker reads out content." .

### Individuals

:InFrontOfMirror rdf:type :UserLocation ;
                  rdfs:label "In front of mirror" ;
                  rdfs:comment "The user location in front of the smart mirror." .

:WalkingAround rdf:type :UserLocation ;
                rdfs:label "Walking around" ;
                rdfs:comment "The user location when walking around the bathroom." .

:BrushingTeeth rdf:type :UserActivity ;
                rdfs:label "Brushing teeth" ;
                rdfs:comment "The user activity of brushing teeth." .

### Restrictions

:SmartMirror rdf:type owl:Class ;
              rdfs:subClassOf [ rdf:type owl:Restriction ;
                                owl:onProperty :displaysContent ;
                                owl:someValuesFrom :WeatherContent ] ;
              rdfs:comment "The smart mirror is capable of displaying weather content as graphics." .

:SmartSpeaker rdf:type owl:Class ;
               rdfs:subClassOf [ rdf:type owl:Restriction ;
                                 owl:onProperty :readsOutContent ;
                                 owl:someValuesFrom :WeatherContent ] ;
               rdfs:comment "The smart speaker is capable of reading out weather content." .

:User rdf:type owl:Class ;
       rdfs:subClassOf [ rdf:type owl:Restriction ;
                         owl:onProperty :hasLocation ;
                         owl:someValuesFrom :UserLocation ] ;
       rdfs:subClassOf [ rdf:type owl:Restriction ;
                         owl:onProperty :hasActivity ;
                         owl:someValuesFrom :UserActivity ] ;
       rdfs:comment "The user has a location and an activity within the smart bathroom." .
